theories/typing/lib/rwlock/rwlockwriteguard.v
@@ -18,7 +18,7 @@ Section rwlockwriteguard.
 
   Program Definition rwlockwriteguard (α : lft) (ty : type) :=
     {| ty_size := 1;
-       ty_lfts := α :: ty.(ty_lfts); ty_E := ty.(ty_E) ++ ty_outlives_E ty α;
+       ty_lfts := α :: ty.(ty_lfts); ty_E := ty.(ty_E) ++ ty_outlv_E ty α;
        ty_own tid vl :=
          match vl return _ with
          | [ #(LitLoc l) ] =>
@@ -71,7 +71,7 @@ Section rwlockwriteguard.
     split.
     - apply (type_lft_morphism_add _ α [α] []) => ?.
       + iApply lft_equiv_refl.
-      + by rewrite elctx_interp_app elctx_interp_ty_outlives_E
+      + by rewrite elctx_interp_app elctx_interp_ty_outlv_E
                    /elctx_interp /= left_id right_id.
     - done.
     - intros n ty1 ty2 Hsz Hl HE Ho Hs tid [|[[]|][]]=>//=. unfold rwlock_inv.
